theories/class_instances.v
@@ -1,9 +1,12 @@
 From Coq Require Import ZArith Lia ssreflect.
 From stdpp Require Import base.
-From cap_machine Require Import machine_base machine_parameters addr_reg classes.
+From cap_machine Require Import machine_base machine_parameters addr_reg classes logical_mapsto.
 From machine_utils Require Export class_instances.
 
 Instance DecodeInstr_encode `{MachineParameters} (i: instr) :
   DecodeInstr (encodeInstrW i) i.
 Proof. apply decode_encode_instrW_inv. Qed.
 
+Instance DecodeInstrL_encode `{MachineParameters} (i: instr) :
+  DecodeInstrL (encodeInstrWL i) i.
+Proof. apply decode_encode_instrLW_inv. Qed.
